operations/Linearize_alist.thy
@@ -3,9 +3,6 @@ theory Linearize_alist
   keywords "linearize_mrbnf" :: thy_goal
 begin
 
-definition asSS :: "('a \<Rightarrow> 'a) \<Rightarrow> 'a \<Rightarrow> 'a" where
-  "asSS f \<equiv> if |supp f| <o |UNIV :: 'a set| then f else id"
-
 ML_file "../Tools/mrbnf_linearize_tactics.ML"
 ML_file "../Tools/mrbnf_linearize.ML"
 
@@ -20,27 +17,27 @@ lemma "\<And> R (x :: 'a list) y. list_all2 R x y = (\<exists>z. set z \<subsete
     done
   done
 
-definition sameShape_list :: "'a list \<Rightarrow> 'a list \<Rightarrow> bool" where 
-  "sameShape_list x x' \<equiv> list_all2 top x x'"
+definition eq_shape_list :: "'a list \<Rightarrow> 'a list \<Rightarrow> bool" where 
+  "eq_shape_list x x' \<equiv> list_all2 top x x'"
 
 definition nonrep_list :: "'a list \<Rightarrow> bool" where 
-  "nonrep_list x \<equiv> \<forall> x'. sameShape_list x x' \<longrightarrow> (\<exists> f. x' = map f x)"
+  "nonrep_list x \<equiv> \<forall> x'. eq_shape_list x x' \<longrightarrow> (\<exists> f. x' = map f x)"
 
-lemma sameShape_list_alt: "list_all2 top xs xs' = (length xs = length xs')"
+lemma eq_shape_list_alt: "list_all2 top xs xs' = (length xs = length xs')"
   by (simp add: list_all2_conv_all_nth)
 
 lemma ex_not: "((\<forall>x. P x) \<longrightarrow> False) = (\<exists>x. \<not>P x)"
   by simp
 
 lemma "nonrep_list [1::nat, 1, 1] \<longrightarrow> False"
-  apply (unfold nonrep_list_def sameShape_list_def sameShape_list_alt)
+  apply (unfold nonrep_list_def eq_shape_list_def eq_shape_list_alt)
   apply (rule ex_not[THEN iffD2])
   apply (rule exI[of _ "[1, 2, 3]"])
   apply (auto)
   done
 
 lemma "nonrep_list [1::nat, 2, 3]"
-  apply (unfold nonrep_list_def sameShape_list_def sameShape_list_alt)
+  apply (unfold nonrep_list_def eq_shape_list_def eq_shape_list_alt)
   apply (rule allI)
   apply (rule impI)
   subgoal for x
@@ -50,22 +47,20 @@ lemma "nonrep_list [1::nat, 2, 3]"
   done
 
 (* PROD *)
-print_bnfs
-
-definition sameShape_prod_1 :: "('a \<times> 'b) \<Rightarrow> ('a \<times> 'b) \<Rightarrow> bool" where 
-  "sameShape_prod_1 x x' \<equiv> rel_prod top (=) x x'"
+definition eq_shape_prod_1 :: "('a \<times> 'b) \<Rightarrow> ('a \<times> 'b) \<Rightarrow> bool" where 
+  "eq_shape_prod_1 x x' \<equiv> rel_prod top (=) x x'"
 
 definition nonrep_prod_1 :: "('a \<times> 'b) \<Rightarrow> bool" where 
-  "nonrep_prod_1 x \<equiv> \<forall> x'. sameShape_prod_1 x x' \<longrightarrow> (\<exists> f. x' = map_prod f id x)"
+  "nonrep_prod_1 x \<equiv> \<forall> x'. eq_shape_prod_1 x x' \<longrightarrow> (\<exists> f. x' = map_prod f id x)"
 
 lemma "nonrep_prod_1 (a, b)"
-  apply (unfold nonrep_prod_1_def sameShape_prod_1_def)
+  apply (unfold nonrep_prod_1_def eq_shape_prod_1_def)
   apply (auto)
   done
 
 typedef 'a nrp_list = "{(xs :: 'a list). nonrep_list xs}"
   apply (rule exI[of _ "[]"])
-  apply (auto simp add: nonrep_list_def sameShape_list_def)
+  apply (auto simp add: nonrep_list_def eq_shape_list_def)
   done
 
 thm fun.set_bd
@@ -89,6 +84,36 @@ bnf "'a set"
   done
 print_theorems
 *)
+
+print_bnfs
+
+definition dom_map :: "('a \<Rightarrow> 'a) \<Rightarrow> ('a \<Rightarrow> 'b) \<Rightarrow> ('a \<Rightarrow> 'b)" where
+  "dom_map g f = f o g"
+
+definition fun_map :: "('a \<Rightarrow> 'a) \<Rightarrow> ('b \<Rightarrow> 'b') \<Rightarrow> ('a \<Rightarrow> 'b) \<Rightarrow> ('a \<Rightarrow> 'b')" where
+  "fun_map d r f = r o f o (inv d)"
+
+definition domain :: "('a \<Rightarrow> 'b) \<Rightarrow> 'a set" where
+  "domain _ = UNIV"
+
+
+mrbnf "('a::var) \<Rightarrow> 'b"
+  map: fun_map
+    sets: bound: domain live: range
+  bd: "natLeq"
+  rel: "rel_fun (=)"
+  subgoal
+    apply (unfold fun_map_def o_id id_o inv_id)
+    apply (unfold id_apply)
+    apply (rule refl)
+    done
+  subgoal for f1 g1 f2 g2
+    apply (unfold fun_map_def o_apply)
+    apply (intro ext)
+    oops
+  
+  
+
 mrbnf "'a list"
   map: map
     sets: set
@@ -246,8 +271,6 @@ mrbnf pre_alist: "('k, 'v) pre_alist"
 
 print_theorems
 
-
-
 linearize_mrbnf ('k::var,'v) alist = "('k::var, 'v) pre_alist" on 'k
   oops
 
@@ -287,7 +310,6 @@ lemma pre_alist_strong:
     apply (insert spec2[OF prems(1), of l z])
     apply (erule impE, intro conjI prems)
     apply (erule impE, intro conjI prems)
-
     apply (rule exI)
     apply (unfold inf_fun_def inf_bool_def)
     apply (rule conjI)
@@ -303,339 +325,114 @@ lemma pre_alist_strong:
     done
   done
 
-ML \<open>
-open BNF_Util BNF_Tactics
-
-fun mk_rel_F_exchange_tac mrbnf F_mr_rel_mono_strong0 F_strong ctxt =
-  let
-    val id_prems = MRBNF_Comp_Tactics.mk_id_prems mrbnf;
-  in
-    HEADGOAL (Subgoal.FOCUS
-      (fn {prems, context = ctxt, ...} => 
-        HEADGOAL (EVERY' [
-          rtac ctxt (F_mr_rel_mono_strong0 OF flat (replicate 2 id_prems)),
-          rtac ctxt (F_strong OF prems),
-          K (unfold_thms_tac ctxt ([id_apply, eqTrueI OF [refl]] @ @{thms ball_triv inf_apply inf_bool_def}))
-        ]) THEN
-        ALLGOALS (
-          (rtac ctxt impI THEN' 
-          rtac ctxt TrueI) ORELSE'
-          (rtac ctxt ballI THEN' 
-          rtac ctxt ballI THEN'
-          rtac ctxt impI THEN'
-          eresolve_tac ctxt [conjunct1, conjunct2]))
-       ) ctxt)
-  end
-\<close>
-
-(* lin_pos dependent? *)
 (* Another important consequence: the following "exchange"-property, which could be read: 
 Since the atoms have a fixed position, we can permute the relations: *)
 lemma rel_F_exchange: 
-  fixes x :: "('a1::var,'a2::var,'a3,'a4) F" and x' :: "('a1,'a2,'a3','a4') F"
-  assumes "rel_F id id R3 R4 x x'" and "rel_F id id Q3 Q4 x x'"
-  shows "rel_F id id R3 Q4 x x'" 
-  using assms apply -
-  apply (tactic \<open>mk_rel_F_exchange_tac (MRBNF_Def.mrbnf_of @{context} @{type_name F} |> the) 
-    @{thm F.mr_rel_mono_strong0} @{thm F_strong} @{context} 
-    THEN print_tac @{context} "done" THEN no_tac\<close>)
-  subgoal premises prems
-    apply (rule F.mr_rel_mono_strong0[OF supp_id_bound bij_id supp_id_bound supp_id_bound bij_id supp_id_bound])
-    apply (rule F_strong[OF prems])
+  fixes x :: "('k, 'v) pre_alist" and x' :: "('k', 'v') pre_alist"
+  assumes "mr_rel_pre_alist Rk Rv x x'" and "mr_rel_pre_alist Qk Qv x x'"
+  shows "mr_rel_pre_alist Rk Qv x x'" 
+    apply (rule pre_alist.mr_rel_mono_strong0)
+    apply (rule pre_alist_strong[OF assms])
        apply (unfold id_apply eqTrueI[OF refl] ball_triv inf_apply inf_bool_def)
-       apply (intro impI TrueI)+
      apply (intro ballI impI; erule conjunct1 conjunct2)+
-    done
   done
 
 (* Then notion of two items having the same shape (w.r.t. the 3rd position): *)
 (* these definitions are lin_pos dependent *)
-definition sameShape1 :: "('a1::var,'a2::var,'a3,'a4) F \<Rightarrow> ('a1,'a2,'a3,'a4) F \<Rightarrow> bool" where 
-  "sameShape1 x x' \<equiv> rel_F id id top (=) x x'"
+definition eq_shape :: "('k, 'v) pre_alist \<Rightarrow> ('k, 'v) pre_alist \<Rightarrow> bool" where 
+  "eq_shape x x' \<equiv> mr_rel_pre_alist top (=) x x'"
 
-definition nonrep2 :: "('a1::var,'a2::var,'a3,'a4) F \<Rightarrow> bool" where 
-  "nonrep2 x \<equiv> \<forall> x'. sameShape1 x x' \<longrightarrow> (\<exists> f. x' = map_F id id f id x)"
+definition nonrep :: "('k, 'v) pre_alist \<Rightarrow> bool" where 
+  "nonrep x \<equiv> \<forall> x'. eq_shape x x' \<longrightarrow> (\<exists> f. x' = map_pre_alist f id x)"
 
-ML\<open>
-open BNF_Util BNF_Tactics
-
-fun mk_nonrep2_map_F_tac mrbnf nonrep_def sameShape_def F_map_comp F_mr_rel_map mr_rel_F_def F_rel_compp 
-  F_rel_Grp F_map_id F_in_rel F_rel_maps F_rel_refl_strong ctxt = 
-  HEADGOAL (Subgoal.FOCUS 
-    (fn {prems, context = ctxt, ...} => 
-      let
-        val var_types = var_types_of_mrbnf mrbnf;
-        val nr_lives = length (filter (fn v => v = MRBNF_Def.Live_Var) var_types);
-        val nr_non_lives = length (filter (fn v => not (v = MRBNF_Def.Live_Var)) var_types);
-        val lin_live_pos = fold_index (fn (i, v) => fn b => 
-          if (v = MRBNF_Def.Live_Var andalso i+1 < lin_pos) then b+1 else b) var_types 1;
-        val switch_poses = map_range (fn i => if i < (lin_pos-(lin_live_pos)) then i+1 else i+2) (nr_non_lives);
-        val switch = (fn thm1 => (fn thm2 => trans OF [thm1, thm2 RS sym]));
-        val o_id = @{thm o_id};
-        val id_o = @{thm id_o};
-      in
-        unfold_thms_tac ctxt [nonrep_def, sameShape_def] THEN
-        HEADGOAL (EVERY' [
-          rtac ctxt allI,
-          rtac ctxt impI,
-          etac ctxt exE,
-          EqSubst.eqsubst_tac ctxt [0] [F_map_comp] THEN_ALL_NEW
-            TRY o resolve_tac ctxt (prems @ @{thms supp_id_bound bij_id}),
-          K (unfold_thms_tac ctxt [switch id_o o_id]),
-          EqSubst.eqsubst_tac ctxt [lin_pos] [switch o_id id_o], (*move all id to the right except for lin_pos*)
-          EqSubst.eqsubst_tac ctxt [0] [F_map_comp RS sym] THEN_ALL_NEW
-            TRY o resolve_tac ctxt (prems @ @{thms supp_id_bound bij_id}),
-          dtac ctxt (rotate_prems ~1 (F_mr_rel_map RS iffD1)) THEN_ALL_NEW
-            TRY o resolve_tac ctxt (prems @ @{thms supp_id_bound bij_id}),
-          K (unfold_thms_tac ctxt [switch id_o o_id, @{thm Grp_UNIV_id}]),
-          K (unfold_thms_tac ctxt [switch @{thm OO_eq} @{thm eq_OO}]),  
-          EqSubst.eqsubst_asm_tac ctxt [lin_live_pos] [switch @{thm eq_OO} @{thm OO_eq}], (*move all (=) to the left except for lin_live_pos*)
-          K (unfold_thms_tac ctxt @{thms eq_alt}),   
-          EqSubst.eqsubst_tac ctxt [0] @{thms Grp_UNIV_id}
-        ]) THEN
-        unfold_thms_tac ctxt [mr_rel_F_def, o_id, F_rel_compp, F_rel_Grp] THEN
-        unfold_thms_tac ctxt [eqTrueI OF @{thms subset_UNIV}, @{thm simp_thms(21)}, id_o, @{thm UNIV_def} RS sym] THEN
-        unfold_thms_tac ctxt ([eqTrueI OF [@{thm UNIV_I}], id_apply] @ @{thms Grp_UNIV_id OO_def Grp_def simp_thms(21)}) THEN
-        HEADGOAL (EVERY' [
-          etac ctxt exE,
-          etac ctxt conjE,
-          dtac ctxt (rotate_prems ~1 (F_in_rel RS iffD1)) THEN_ALL_NEW
-            TRY o resolve_tac ctxt prems,
-          Method.insert_tac ctxt [unfold_thms ctxt [nonrep_def, sameShape_def, mr_rel_F_def, F_map_id] 
-            (nth prems (length prems -1))],
-          etac ctxt exE,
-          etac ctxt conjE,
-          etac ctxt CollectE,
-          etac ctxt conjE
-        ]) THEN
-        REPEAT_DETERM_N (nr_lives-1) (HEADGOAL (
-          etac ctxt conjE)) THEN
-        HEADGOAL (hyp_subst_tac_thin true ctxt) THEN
-        HEADGOAL (Subgoal.FOCUS 
-          (fn {prems = subprems, context = ctxt, params, ...} => 
-            HEADGOAL (EVERY' [
-              Method.insert_tac ctxt [nth subprems 0],
-              etac ctxt allE,
-              etac ctxt impE,
-              rtac ctxt (infer_instantiate' ctxt [NONE, SOME (snd (nth params 1))] exI),
-              EqSubst.eqsubst_tac ctxt [1] [nth F_rel_maps 0],
-              EqSubst.eqsubst_tac ctxt [1] [nth F_rel_maps 1]
-            ]) THEN
-            HEADGOAL (rtac ctxt F_rel_refl_strong) THEN
-            REPEAT_DETERM_N nr_lives (HEADGOAL (
-                (dresolve_tac ctxt (map (fn p => subsetD OF [p] RS @{thm Collect_case_prodD}) (drop 1 subprems)) THEN'
-                  (assume_tac ctxt ORELSE' 
-                  (rtac ctxt sym THEN' assume_tac ctxt))))) THEN
-            HEADGOAL (EVERY' [
-              etac ctxt exE,
-              EqSubst.eqsubst_tac ctxt [0] [F_map_comp] THEN_ALL_NEW
-                TRY o resolve_tac ctxt (prems @ @{thms supp_id_bound bij_id}),
-              EqSubst.eqsubst_tac ctxt switch_poses [switch id_o o_id],
-              EqSubst.eqsubst_tac ctxt [0] [F_map_comp RS sym] THEN_ALL_NEW
-                TRY o resolve_tac ctxt (prems @ @{thms supp_id_bound bij_id}),
-              rtac ctxt exI,
-              dtac ctxt arg_cong,
-              assume_tac ctxt
-            ]) 
-          ) ctxt)
-      end)
-  ctxt)
-\<close>
-
-lemma nonrep2_map_F:
-  fixes x :: "('a1::var,'a2::var,'a3,'a4) F"
-    and v :: "'a1 \<Rightarrow> 'a1" and u :: "'a2\<Rightarrow>'a2" and g :: "'a4 \<Rightarrow> 'b4"
-  assumes v: "|supp v| <o |UNIV :: 'a1 set|"  and u: "bij u" "|supp u| <o |UNIV :: 'a2 set|" 
-  assumes "nonrep2 x"
-  shows "nonrep2 (map_F v u id g x)"
-  using assms apply -
-  subgoal premises prems
-    apply (unfold nonrep2_def sameShape1_def)
-    apply (rule allI)
-    apply (rule impI)
-    apply (subst F.map_comp; (rule prems bij_id supp_id_bound)?)
-    apply (unfold o_id id_o)
-    apply (drule iffD1[OF F.mr_rel_map(1), rotated -1]; (rule prems bij_id supp_id_bound)?)
-    apply (unfold trans[OF id_o o_id[symmetric]] Grp_UNIV_id trans[OF OO_eq eq_OO[symmetric]])
-    apply (unfold trans[OF eq_OO OO_eq[symmetric], of top])
-    apply (unfold eq_alt)
-    apply (subst Grp_UNIV_id)
-    apply (unfold mr_rel_F_def o_id F.rel_compp F.rel_Grp)
-    apply (unfold eqTrueI[OF subset_UNIV] simp_thms(21) UNIV_def[symmetric] id_o)
-    apply (unfold Grp_UNIV_id OO_def Grp_def eqTrueI[OF UNIV_I] simp_thms(21) id_apply)
-    apply (unfold id_def[THEN sym])
-    apply (erule exE)
-    apply (erule conjE)
-    apply (drule F.in_rel[THEN iffD1, rotated -1]; (rule prems)?)
-    apply (erule exE)
-    apply (erule conjE)
-    apply (erule CollectE)
-    apply (erule conjE)
-    apply (erule conjE)
-    apply (insert prems(4)[unfolded nonrep2_def sameShape1_def mr_rel_F_def F.map_id])
-    apply (rotate_tac -1)
-    apply (hypsubst_thin)
-    subgoal premises subprems for x' y z
-      apply (insert subprems(1))
-      apply (erule allE)
-      apply (erule impE)
-       apply (subst F.rel_map)
-       apply (subst F.rel_map)
-       apply (rule F.rel_refl_strong)
-        apply (drule subsetD[OF subprems(2), THEN Collect_case_prodD] 
-          subsetD[OF subprems(3), THEN Collect_case_prodD]; 
-          (assumption)?; (rule sym; assumption)?)+
-      apply (elim exE)
-      apply (subst F.map_comp[OF _ _ _ supp_id_bound bij_id supp_id_bound, unfolded trans[OF id_o o_id[symmetric]]]; (rule prems)?)
-      apply (subst F.map_comp[THEN sym]; (rule prems bij_id supp_id_bound)?)
-      subgoal premises subprems for f
-        apply (rule exI[of _ f]) (* instantiation not necessary but easy*)
-        apply (subst subprems)
-        apply (subst F.map_comp; (rule prems bij_id supp_id_bound)?)
-        apply (unfold o_id id_o)
-        apply (rule refl)
-        done
+lemma nonrep_map_F:
+  fixes x :: "('k, 'v) pre_alist" and g :: "'v \<Rightarrow> 'v"
+  assumes "nonrep x"
+  shows "nonrep (map_pre_alist id g x)"
+  apply (unfold nonrep_def eq_shape_def)
+  apply (rule allI)
+  apply (rule impI)
+  apply (subst pre_alist.map_comp; (rule assms bij_id supp_id_bound)?)
+  apply (unfold o_id id_o)
+  apply (drule iffD1[OF pre_alist.mr_rel_map(1), rotated -1])
+  apply (unfold trans[OF id_o o_id[symmetric]] Grp_UNIV_id trans[OF OO_eq eq_OO[symmetric]])
+  apply (unfold trans[OF eq_OO OO_eq[symmetric], of top])
+  apply (unfold eq_alt)
+  apply (subst Grp_UNIV_id)
+  apply (unfold mr_rel_pre_alist_def o_id pre_alist.rel_compp pre_alist.rel_Grp)
+  apply (unfold eqTrueI[OF subset_UNIV] simp_thms(21) UNIV_def[symmetric] id_o)
+  apply (unfold Grp_UNIV_id OO_def Grp_def eqTrueI[OF UNIV_I] simp_thms(21) id_apply)
+  apply (unfold id_def[THEN sym])
+  apply (erule exE)
+  apply (erule conjE)
+  apply (drule pre_alist.in_rel[THEN iffD1, rotated -1])
+  apply (erule exE)
+  apply (erule conjE)
+  apply (erule CollectE)
+  apply (erule conjE)
+  apply (erule conjE)
+  apply (insert assms(1)[unfolded nonrep_def eq_shape_def mr_rel_pre_alist_def pre_alist.map_id])
+  apply (rotate_tac -1)
+  apply (hypsubst_thin)
+  subgoal premises prems for x' y z
+    apply (insert prems(1))
+    apply (erule allE)
+    apply (erule impE)
+     apply (subst pre_alist.rel_map)
+     apply (subst pre_alist.rel_map)
+     apply (rule pre_alist.rel_refl_strong)
+      apply (drule subsetD[OF prems(2), THEN Collect_case_prodD] 
+        subsetD[OF prems(3), THEN Collect_case_prodD]; 
+        (assumption)?; (rule sym; assumption)?)+
+    apply (elim exE)
+    apply (subst pre_alist.map_comp[unfolded trans[OF id_o o_id[symmetric]]])
+    apply (subst pre_alist.map_comp[THEN sym]; (rule prems bij_id supp_id_bound)?)
+    subgoal premises subprems for f
+      apply (rule exI[of _ f]) (* instantiation not necessary but easy *)
+      apply (subst subprems)
+      apply (subst pre_alist.map_comp; (rule prems bij_id supp_id_bound)?)
+      apply (unfold o_id id_o)
+      apply (rule refl)
       done
     done
   done
 
-ML\<open>
-open BNF_Util BNF_Tactics
-
-fun mk_nonrep2_map_F_rev_tac mrbnf nonrep_def sameShape_def F_mr_rel_map1 F_mr_rel_map2 F_mr_rel_map3 F_map_comp F_rel_eq 
-  F_mr_rel_id rel_F_exchange F_mr_rel_flip F_mr_rel_mono_strong0 F_mr_rel_Grp ctxt = 
-  HEADGOAL (Subgoal.FOCUS 
-    (fn {prems, context = ctxt, ...} => 
-      let
-        val var_types = var_types_of_mrbnf mrbnf;
-        val nr_lives = length (filter (fn v => v = MRBNF_Def.Live_Var) var_types);
-        val nr_non_lives = length (filter (fn v => not (v = MRBNF_Def.Live_Var)) var_types);
-        val lin_live_pos = fold_index (fn (i, v) => fn b => 
-          if (v = MRBNF_Def.Live_Var andalso i+1 < lin_pos) then b+1 else b) var_types 1;
-        val switch = (fn thm1 => (fn thm2 => trans OF [thm1, thm2 RS sym]));
-      in
-        unfold_thms_tac ctxt [nonrep_def, sameShape_def] THEN
-        HEADGOAL (EVERY' [
-          rtac ctxt allI,
-          rtac ctxt impI,
-          etac ctxt exE,
-          forward_tac ctxt [rotate_prems ~1 F_mr_rel_map2] THEN_ALL_NEW
-            TRY o resolve_tac ctxt (prems @ @{thms supp_id_bound bij_id}),
-          rotate_tac 1,
-          EqSubst.eqsubst_asm_tac ctxt (map_range (fn i => i+1) nr_non_lives) [switch @{thm o_id} @{thm id_o}],
-          EqSubst.eqsubst_asm_tac ctxt [lin_live_pos] @{thms Grp_UNIV_id},
-          K (unfold_thms_tac ctxt [switch @{thm eq_OO} @{thm OO_eq}]),
-          EqSubst.eqsubst_asm_tac ctxt [lin_live_pos] [switch @{thm OO_eq} @{thm eq_OO}], (*move all (=) to the right and then lin_live_pos back*)
-          EqSubst.eqsubst_asm_tac ctxt [lin_live_pos] @{thms eq_alt},
-          EqSubst.eqsubst_asm_tac ctxt [0] [F_mr_rel_map1 RS sym] THEN_ALL_NEW
-            TRY o resolve_tac ctxt (prems @ @{thms supp_id_bound bij_id}),
-          Method.insert_tac ctxt [unfold_thms ctxt [nonrep_def, sameShape_def] (nth prems (length prems - 1))],
-          etac ctxt allE,
-          etac ctxt impE,
-          rtac ctxt exI,
-          assume_tac ctxt,
-          etac ctxt thin_rl,
-          etac ctxt exE,
-          EqSubst.eqsubst_asm_tac ctxt [0] [F_map_comp] THEN_ALL_NEW
-            TRY o resolve_tac ctxt (prems @ @{thms supp_id_bound bij_id}),
-          K (unfold_thms_tac ctxt @{thms id_o o_id}),
-          EqSubst.eqsubst_asm_tac ctxt [1] [F_rel_eq RS sym],
-          EqSubst.eqsubst_asm_tac ctxt [1] [F_mr_rel_id],
-          dtac ctxt (rotate_prems ~1 (iffD1 OF [F_mr_rel_map1])) THEN_ALL_NEW
-            TRY o resolve_tac ctxt (prems @ @{thms supp_id_bound bij_id}),
-          K (unfold_thms_tac ctxt @{thms id_o OO_eq}),
-          dtac ctxt (rotate_prems 1 rel_F_exchange),
-          rtac ctxt (F_mr_rel_flip RS iffD1) THEN_ALL_NEW
-            TRY o resolve_tac ctxt @{thms supp_id_bound bij_id},
-          K (unfold_thms_tac ctxt @{thms inv_id}),
-          EqSubst.eqsubst_asm_tac ctxt [0] [F_mr_rel_map3] THEN_ALL_NEW
-            TRY o resolve_tac ctxt (prems @ @{thms supp_id_bound bij_id}),
-          EqSubst.eqsubst_asm_tac ctxt (map_range (fn i => i+1) (2 * nr_lives)) @{thms Grp_def},
-          EqSubst.eqsubst_asm_tac ctxt (map_range (fn i => i+1) (nr_non_lives)) @{thms inv_o_simp1} THEN_ALL_NEW
-            TRY o resolve_tac ctxt (@{thm bij_id}::prems),
-          K (unfold_thms_tac ctxt ((eqTrueI OF @{thms UNIV_I}):: @{thms id_apply simp_thms(21)})),
-          EqSubst.eqsubst_asm_tac ctxt [lin_live_pos] @{thms eq_commute},
-          K (unfold_thms_tac ctxt @{thms eq_OO conversep_def}),
-          etac ctxt (rotate_prems (~1 - (length var_types)) F_mr_rel_mono_strong0) THEN_ALL_NEW
-            TRY o resolve_tac ctxt @{thms supp_id_bound bij_id}
-        ]) THEN
-        REPEAT_DETERM_N (length var_types) (
-          (HEADGOAL (
-            (* for bound and free *)
-            rtac ctxt ballI THEN'
-            rtac ctxt refl)) 
-          ORELSE 
-          (HEADGOAL (
-            (* for lives*)
-            rtac ctxt ballI THEN'
-            rtac ctxt ballI THEN'
-            rtac ctxt impI THEN'
-            rotate_tac 2 THEN'
-            EqSubst.eqsubst_asm_tac ctxt [0] @{thms eq_commute} THEN'
-            assume_tac ctxt))
-        ) THEN
-        HEADGOAL (EVERY' [
-          etac ctxt thin_rl,
-          EqSubst.eqsubst_asm_tac ctxt [lin_live_pos] [@{thm Grp_UNIV_def} RS sym],
-          rtac ctxt exI,
-          EqSubst.eqsubst_asm_tac ctxt (map_range (fn i => i+1) (nr_lives -1)) @{thms eq_alt},
-          EqSubst.eqsubst_asm_tac ctxt [0] [F_mr_rel_Grp] THEN_ALL_NEW
-            TRY o resolve_tac ctxt @{thms supp_id_bound bij_id}
-        ]) THEN
-        unfold_thms_tac ctxt ([eqTrueI OF @{thms subset_UNIV}, eqTrueI OF @{thms UNIV_I}, @{thm UNIV_def} RS sym] @ 
-          @{thms simp_thms(21) Grp_def}) THEN
-        HEADGOAL (assume_tac ctxt)
-      end)
-  ctxt)
-\<close>
 
 (* Here we need pullback preservation: *)
-lemma nonrep2_map_F_rev:
-  fixes x :: "('a1::var,'a2::var,'a3,'a4) F" and u :: "'a2\<Rightarrow>'a2" and g :: "'a4 \<Rightarrow> 'a4'"
-  assumes u: "bij u" "|supp u| <o |UNIV :: 'a2 set|" 
-  assumes "nonrep2 (map_F id u id g x)"
-  shows "nonrep2 x"
+lemma nonrep_map_F_rev:
+  fixes x :: "('k, 'v) pre_alist" and g :: "'v \<Rightarrow> 'v'"
+  assumes "nonrep (map_pre_alist id g x)"
+  shows "nonrep x"
   using assms apply -
- (* apply (tactic \<open>mk_nonrep2_map_F_rev_tac (MRBNF_Def.mrbnf_of @{context} @{type_name F} |> the) @{thm nonrep2_def} @{thm sameShape1_def} @{thm F.mr_rel_map(1)}
-    @{thm F.mr_rel_map(2)} @{thm F.mr_rel_map(3)} @{thm F.map_comp} @{thm F.rel_eq} @{thm F.mr_rel_id} @{thm rel_F_exchange} 
-    @{thm F.mr_rel_flip} @{thm F.mr_rel_mono_strong0} @{thm F.mr_rel_Grp} @{context} 
-    THEN print_tac @{context} "done" THEN no_tac\<close>)*)
   subgoal premises prems
-    apply (unfold nonrep2_def sameShape1_def)
+    apply (unfold nonrep_def eq_shape_def)
     apply (rule allI)
     apply (rule impI)
 
 (* alt *)
-    apply (insert prems(3)[unfolded nonrep2_def sameShape1_def]) (*lastprem*)
+    apply (insert prems(1)[unfolded nonrep_def eq_shape_def])
     apply (elim allE impE)
-     apply (rule F.mr_rel_map(1)[THEN iffD2]; (rule prems supp_id_bound bij_id)?)
-  (*_ * (2*nr_BF + nr_As + 2(x,y)) *)
-   apply (drule F.mr_rel_map(2)[rotated -1, of _ _ _ _ _ _ _ _ id _]; (rule prems supp_id_bound bij_id)?)
+     apply (rule pre_alist.mr_rel_map(1)[THEN iffD2]; (rule prems supp_id_bound bij_id)?)
+     apply (drule pre_alist.mr_rel_map(2)[rotated -1, of _ _ _ _ id])
      apply (unfold o_id id_o Grp_UNIV_id eq_OO OO_eq)
      apply (assumption)
 
     apply (erule exE)
-    apply (subst (asm) F.map_comp; (rule prems supp_id_bound bij_id)?)
+    apply (subst (asm) pre_alist.map_comp; (rule prems supp_id_bound bij_id)?)
     apply (unfold o_id id_o)
 
-    thm F.map_cong
-
-    apply (subst (asm) F.rel_eq[symmetric])
-    apply (unfold F.mr_rel_id)
-    thm F.mr_rel_map
-    apply (drule iffD1[OF F.mr_rel_map(1), rotated -1]; (rule prems supp_id_bound bij_id)?)
+    apply (subst (asm) pre_alist.rel_eq[symmetric])
+    apply (unfold pre_alist.mr_rel_id)
+    apply (drule iffD1[OF pre_alist.mr_rel_map(1), rotated -1]; (rule prems supp_id_bound bij_id)?)
     apply (unfold id_o OO_eq)
-    thm rel_F_exchange[rotated]
     apply (drule rel_F_exchange[rotated])
-     apply (rule iffD1[OF F.mr_rel_flip]; (rule supp_id_bound bij_id)?)
-    apply (unfold inv_id)
-     apply (subst (asm) F.mr_rel_map(3); (rule prems supp_id_bound bij_id)?)
+     apply (rule iffD1[OF pre_alist.mr_rel_flip])
+     apply (subst (asm) pre_alist.mr_rel_map(3))
      apply (unfold Grp_def)
-    apply (subst (asm) (1 2) inv_o_simp1; (rule prems bij_id)?) (*for all frees and bounds*)
-     apply (tactic \<open>unfold_thms_tac @{context} @{thms eqTrueI[OF UNIV_I] simp_thms(21) id_apply}\<close>) (*for all frees*)
+     apply (tactic \<open>Ctr_Sugar_Tactics.unfold_thms_tac @{context} @{thms eqTrueI[OF UNIV_I] simp_thms(21) id_apply}\<close>)
      apply (subst (asm) eq_commute) (*lin_live_pos*)
      apply (unfold eq_OO conversep_def)
-     apply (elim F.mr_rel_mono_strong0[rotated -5]; (rule supp_id_bound bij_id)?) (*- len vartypes - 1*)
+     apply (elim pre_alist.mr_rel_mono_strong0) (*- len vartypes - 1*)
       (*left subtactic is for frees and bounds, right subtactic for lives*)
     apply ((rule ballI,rule refl)?; (rule ballI,rule ballI,rule impI,rotate_tac 2,subst (asm) eq_commute,assumption))+
 
@@ -643,135 +440,68 @@ lemma nonrep2_map_F_rev:
     apply (subst (asm) Grp_UNIV_def[symmetric]) (*lin_live_pos*)
     apply (rule exI)
     apply (subst (asm) eq_alt) (* repeat lives - 1 *)
-    thm F.mr_rel_Grp
-    apply (subst (asm) F.mr_rel_Grp; (rule supp_id_bound bij_id)?)
+    apply (subst (asm) pre_alist.mr_rel_Grp)
     apply (unfold eqTrueI[OF subset_UNIV] eqTrueI[OF UNIV_I] UNIV_def[THEN sym] simp_thms(21) Grp_def)
     apply (assumption)
     done
   done
 
-ML\<open>
-open BNF_Util BNF_Tactics
-fun mk_nonrep2_map_bij_tac nonrep_def sameShape_def F_mr_rel_map1 F_map_comp cgs ctxt = 
-  HEADGOAL (Subgoal.FOCUS 
-    (fn {prems, context = ctxt, ...} => 
-      unfold_thms_tac ctxt [nonrep_def, sameShape_def] THEN
-      HEADGOAL (EVERY' [
-        rtac ctxt allI,
-        rtac ctxt impI,
-        dtac ctxt (rotate_prems ~1 (F_mr_rel_map1 RS iffD1)) THEN_ALL_NEW
-          TRY o resolve_tac ctxt @{thms bij_id supp_id_bound},
-        K (unfold_thms_tac ctxt @{thms o_id Grp_UNIV_id eq_OO Grp_OO_top}),
-        dtac ctxt (Object_Logic.rulify ctxt (unfold_thms ctxt [nonrep_def, sameShape_def] (nth prems 1))),
-        etac ctxt exE,
-        hyp_subst_tac_thin true ctxt
-      ]) THEN
-      unfold_thms_tac ctxt @{thms triv_forall_equality} THEN
-      HEADGOAL (Subgoal.FOCUS 
-        (fn {context = ctxt, params, ...} => 
-          HEADGOAL (EVERY' (map (fn ((_, cf), cg) => 
-            let
-              val g = Thm.term_of cg
-              val (dom_g, rng_g) = fastype_of g |> dest_funT
-              val inv_g = Const ("Hilbert_Choice.inv", 
-                (fastype_of g) --> (rng_g --> dom_g)) $ g
-              val f_o_inv_g = HOLogic.mk_comp (Thm.term_of cf, inv_g)
-            in
-              rtac ctxt (infer_instantiate' ctxt [NONE, SOME (Thm.cterm_of ctxt f_o_inv_g)] exI) 
-            end) (params ~~ cgs))
-          ) THEN
-          HEADGOAL (rtac ctxt sym) THEN
-          HEADGOAL (rtac ctxt trans) THEN
-          HEADGOAL (rtac ctxt F_map_comp THEN_ALL_NEW
-            TRY o resolve_tac ctxt @{thms bij_id supp_id_bound}) THEN
-          unfold_thms_tac ctxt ([@{thm inv_o_simp1} OF (take 1 prems), @{thm o_assoc} RS sym] @ @{thms id_o o_id}) THEN
-          HEADGOAL (rtac ctxt refl)
-        ) ctxt)
-  ) ctxt)
-\<close>
-
-lemma nonrep2_mapF_bij:
-  fixes x :: "('a1::var,'a2::var,'a3,'a4) F" and g::"'a3\<Rightarrow>'a3"
-  assumes g: "bij g" and x: "nonrep2 x"
-  shows "nonrep2 (map_F id id g id x)" (is "nonrep2 ?x'")
+lemma nonrep_mapF_bij:
+  fixes x :: "('k, 'v) pre_alist" and g::"'k \<Rightarrow> 'k"
+  assumes g: "bij g" and x: "nonrep x"
+  shows "nonrep (map_pre_alist g id x)"
   using assms apply -
-  apply (tactic \<open>mk_nonrep2_map_bij_tac @{thm nonrep2_def}
-    @{thm sameShape1_def} @{thm F.mr_rel_map(1)} @{thm F.map_comp} [@{cterm g}] @{context}
-    THEN print_tac @{context} "done" THEN no_tac\<close>) 
   subgoal premises prems
-    apply (unfold nonrep2_def sameShape1_def)
+    apply (unfold nonrep_def eq_shape_def)
     apply (rule allI)
     apply (rule impI)
-    apply (drule F.mr_rel_map(1)[THEN iffD1, rotated -1]; (rule supp_id_bound bij_id)?)
+    apply (drule pre_alist.mr_rel_map(1)[THEN iffD1, rotated -1]; (rule supp_id_bound bij_id)?)
     apply (unfold o_id Grp_UNIV_id eq_OO Grp_OO_top)
-    apply (drule x[unfolded nonrep2_def sameShape1_def, rule_format])
+    apply (drule x[unfolded nonrep_def eq_shape_def, rule_format])
     apply (erule exE conjE)+
     apply hypsubst_thin
     subgoal for _ f
       apply (rule exI[of _ "f o inv g"])
       apply (rule sym)
       apply (rule trans)
-       apply (rule F.map_comp; (rule supp_id_bound bij_id)?)
+       apply (rule pre_alist.map_comp; (rule supp_id_bound bij_id)?)
       apply (unfold id_o o_id inv_o_simp1[OF g] o_assoc[symmetric])
       apply (rule refl)
       done
     done
   done
 
-ML \<open>
-open BNF_Util BNF_Tactics
-
-fun mk_nonrep2_mapF_bij_2_tac mrbnf nonrep2_mapF_bij nonrep2_map_F F_map_comp ctxt =
-  HEADGOAL (Subgoal.FOCUS
-    (fn {prems, context = ctxt, ...} => 
-    let val nr_prems = length prems;
-        val id_prems = MRBNF_Comp_Tactics.mk_id_prems mrbnf;
-    in
-      HEADGOAL (rtac ctxt (unfold_thms ctxt ((F_map_comp OF ((take (nr_prems-2) prems) @ id_prems)) :: @{thms id_o o_id}) 
-        (nonrep2_mapF_bij OF [nth prems (nr_prems-2), nonrep2_map_F OF (nth_drop (nr_prems-2) prems)])
-      ))
-     end) ctxt)
-\<close>
-
-lemma nonrep2_mapF_bij_2:
-  fixes x :: "('a1::var,'a2::var,'a3,'a4) F"
-    and v :: "'a1 \<Rightarrow> 'a1" and u :: "'a2\<Rightarrow>'a2" and g::"'a3\<Rightarrow>'a3" and f::"'a4\<Rightarrow>'a4'"
-  assumes v: "|supp v| <o |UNIV :: 'a1 set|" and u: "bij u" "|supp u| <o |UNIV :: 'a2 set|"
-    and g: "bij g" and x: "nonrep2 x"
-  shows "nonrep2 (map_F v u g f x)" 
+lemma nonrep_mapF_bij_2:
+  fixes x :: "('k, 'v) pre_alist" and g::"'k \<Rightarrow> 'k" and f::"'v \<Rightarrow> 'v"
+  assumes g: "bij g" and x: "nonrep x"
+  shows "nonrep (map_pre_alist g f x)" 
   using assms apply -
-  apply (tactic \<open>mk_nonrep2_mapF_bij_2_tac (MRBNF_Def.mrbnf_of @{context} @{type_name F} |> the) 
-    @{thm nonrep2_mapF_bij} @{thm nonrep2_map_F} @{thm F.map_comp} @{context} 
-    THEN print_tac @{context} "done" THEN no_tac\<close>)
   subgoal premises prems
-    apply (rule nonrep2_mapF_bij[OF prems(4) nonrep2_map_F[OF prems(1,2,3,5)], 
-          unfolded F.map_comp[OF prems(1,2,3) supp_id_bound bij_id supp_id_bound] id_o o_id])
+    apply (rule nonrep_mapF_bij[OF prems(1) nonrep_map_F[OF prems(2)], 
+          unfolded pre_alist.map_comp id_o o_id])
     done
   done
 
 
-typedef ('a1::var,'a2::var,'a3::var,'a4) F' = "{x :: ('a1,'a2,'a3,'a4) F. nonrep2 x}"
-  apply (unfold mem_Collect_eq nonrep2_def sameShape1_def mr_rel_F_def F.map_id)
+typedef ('k::var,'v) alist = "{x :: ('k, 'v) pre_alist. nonrep x}"
+  apply (unfold mem_Collect_eq nonrep_def eq_shape_def mr_rel_pre_alist_def pre_alist.map_id)
   by (rule ex_nonrep)
 
-definition set1_F' :: "('a1::var,'a2::var,'a3::var,'a4) F' \<Rightarrow> 'a1 set" where "set1_F' = set1_F o Rep_F'"
-definition set2_F' :: "('a1::var,'a2::var,'a3::var,'a4) F' \<Rightarrow> 'a2 set" where "set2_F' = set2_F o Rep_F'"
-definition set3_F' :: "('a1::var,'a2::var,'a3::var,'a4) F' \<Rightarrow> 'a3 set" where "set3_F' = set3_F o Rep_F'"
-definition set4_F' :: "('a1::var,'a2::var,'a3::var,'a4) F' \<Rightarrow> 'a4 set" where "set4_F' = set4_F o Rep_F'"
+definition keys' :: "('k::var, 'v) alist \<Rightarrow> 'k set" where "keys' = keys o Rep_alist"
+definition vals' :: "('k::var, 'v) alist \<Rightarrow> 'v set" where "vals' = vals o Rep_alist"
 
-definition map_F' :: "('a1::var \<Rightarrow> 'a1) \<Rightarrow> ('a2::var \<Rightarrow> 'a2) \<Rightarrow> ('a3::var \<Rightarrow> 'a3) \<Rightarrow> ('a4 \<Rightarrow> 'a4') 
-  \<Rightarrow> ('a1,'a2,'a3,'a4) F' \<Rightarrow> ('a1,'a2,'a3,'a4') F'"
-  where "map_F' v u f g = Abs_F' o map_F (asSS v) (asSS (asBij u)) (asBij f) g o Rep_F'"
+definition map_alist :: "('k::var \<Rightarrow> 'k) \<Rightarrow> ('v \<Rightarrow> 'v') \<Rightarrow> ('k, 'v) alist \<Rightarrow> ('k, 'v') alist"
+  where "map_alist f g = Abs_alist o map_pre_alist (asBij f) g o Rep_alist"
 
-definition rrel_F' :: "('a4 \<Rightarrow> 'a4' \<Rightarrow> bool) \<Rightarrow> ('a1::var,'a2::var,'a3::var,'a4) F' \<Rightarrow> ('a1,'a2,'a3,'a4') F' \<Rightarrow> bool"
-  where "rrel_F' R x x' = rrel_F (=) R (Rep_F' x) (Rep_F' x')"
+definition rrel_alist :: "('v \<Rightarrow> 'v' \<Rightarrow> bool) \<Rightarrow> ('k::var, 'v) alist \<Rightarrow> ('k::var, 'v') alist \<Rightarrow> bool"
+  where "rrel_alist R x x' = rel_pre_alist (=) R (Rep_alist x) (Rep_alist x')"
 
 (* Verifying the axioms of a MRBNF for F':  *)
-lemma F'_map_id: "map_F' id id id id = id"
-  apply (unfold map_F'_def asSS_def asBij_def 
+lemma F'_map_id: "map_alist id id = id"
+  apply (unfold map_alist_def asSS_def asBij_def 
       eqTrueI[OF bij_id] eqTrueI[OF supp_id_bound] if_True)
   apply (rule ext)
-  apply (unfold o_apply F.map_id Rep_F'_inverse)
+  apply (unfold o_apply pre_alist.map_id Rep_alist_inverse)
   apply (unfold id_def)
   apply (rule refl)
   done
@@ -798,7 +528,7 @@ lemma F'_map_comp1_:
     apply (subst F.map_comp0; (rule prems)?)
     apply (unfold o_apply)
     apply (subst Abs_F'_inverse[unfolded mem_Collect_eq])
-     apply (rule nonrep2_mapF_bij_2; (rule prems Rep_F'[unfolded mem_Collect_eq])?)
+     apply (rule nonrep_mapF_bij_2; (rule prems Rep_F'[unfolded mem_Collect_eq])?)
     apply (rule refl)
     done
   done
@@ -808,13 +538,13 @@ lemma F'_map_comp1_:
 ML \<open>
 open BNF_Util BNF_Tactics
 
-fun mk_set_map_tac set_F'_def map_F'_def Abs_F'_inverse Rep_F' nonrep2_mapF_bij_2 F_set_map ctxt =
+fun mk_set_map_tac set_F'_def map_F'_def Abs_F'_inverse Rep_F' nonrep_mapF_bij_2 F_set_map ctxt =
   HEADGOAL (Subgoal.FOCUS
     (fn {prems = prems, context = ctxt, ...} =>
       unfold_thms_tac ctxt ([set_F'_def, map_F'_def] @ map (fn thm => thm RS eqTrueI) prems @
         @{thms asSS_def asBij_def if_True o_apply}) THEN
       HEADGOAL (EVERY' [EqSubst.eqsubst_tac ctxt [0] [Abs_F'_inverse],
-        rtac ctxt nonrep2_mapF_bij_2 THEN_ALL_NEW resolve_tac ctxt (Rep_F' :: prems),
+        rtac ctxt nonrep_mapF_bij_2 THEN_ALL_NEW resolve_tac ctxt (Rep_F' :: prems),
         rtac ctxt F_set_map THEN_ALL_NEW
           resolve_tac ctxt prems])
     ) ctxt)
@@ -830,13 +560,13 @@ lemma F'_set1_map_:
   shows "set1_F' (map_F' u1 u2 u3 f b) = u1 ` set1_F' b"
   using assms apply -
   apply (tactic \<open>mk_set_map_tac @{thm set1_F'_def} @{thm map_F'_def} @{thm Abs_F'_inverse[unfolded mem_Collect_eq]}
-    @{thm Rep_F'[unfolded mem_Collect_eq]} @{thm nonrep2_mapF_bij_2} @{thm F.set_map(1)} @{context} 
+    @{thm Rep_F'[unfolded mem_Collect_eq]} @{thm nonrep_mapF_bij_2} @{thm F.set_map(1)} @{context} 
     THEN print_tac @{context} "done" THEN no_tac\<close>)
   subgoal premises prems
     apply (unfold set1_F'_def map_F'_def asSS_def asBij_def
         eqTrueI[OF prems(1)] eqTrueI[OF prems(2)] eqTrueI[OF prems(3)] eqTrueI[OF prems(4)] eqTrueI[OF prems(5)] o_apply if_True)
     apply (subst Abs_F'_inverse[unfolded mem_Collect_eq])
-     apply (rule nonrep2_mapF_bij_2; (rule prems Rep_F'[unfolded mem_Collect_eq])?)
+     apply (rule nonrep_mapF_bij_2; (rule prems Rep_F'[unfolded mem_Collect_eq])?)
     apply (rule F.set_map(1); (rule prems))
     done
   done
@@ -851,7 +581,7 @@ lemma F'_set2_map_:
   shows "set2_F' (map_F' u1 u2 u3 f b) = u2 ` set2_F' b"
   using assms apply -
   apply (tactic \<open>mk_set_map_tac @{thm set2_F'_def} @{thm map_F'_def} @{thm Abs_F'_inverse[unfolded mem_Collect_eq]}
-    @{thm Rep_F'[unfolded mem_Collect_eq]} @{thm nonrep2_mapF_bij_2} @{thm F.set_map(2)} @{context}\<close>)
+    @{thm Rep_F'[unfolded mem_Collect_eq]} @{thm nonrep_mapF_bij_2} @{thm F.set_map(2)} @{context}\<close>)
   done
 
 lemma F'_set3_map_:
@@ -864,7 +594,7 @@ lemma F'_set3_map_:
   shows "set3_F' (map_F' u1 u2 u3 f b) = u3 ` set3_F' b"
   using assms apply -
   apply (tactic \<open>mk_set_map_tac @{thm set3_F'_def} @{thm map_F'_def} @{thm Abs_F'_inverse[unfolded mem_Collect_eq]}
-    @{thm Rep_F'[unfolded mem_Collect_eq]} @{thm nonrep2_mapF_bij_2} @{thm F.set_map(3)} @{context}\<close>)
+    @{thm Rep_F'[unfolded mem_Collect_eq]} @{thm nonrep_mapF_bij_2} @{thm F.set_map(3)} @{context}\<close>)
   done
 
 lemma F'_set4_map_:
@@ -877,7 +607,7 @@ lemma F'_set4_map_:
   shows "set4_F' (map_F' u1 u2 u3 f b) = f ` set4_F' b"
   using assms apply -
   apply (tactic \<open>mk_set_map_tac @{thm set4_F'_def} @{thm map_F'_def} @{thm Abs_F'_inverse[unfolded mem_Collect_eq]}
-    @{thm Rep_F'[unfolded mem_Collect_eq]} @{thm nonrep2_mapF_bij_2} @{thm F.set_map(4)} @{context}\<close>)
+    @{thm Rep_F'[unfolded mem_Collect_eq]} @{thm nonrep_mapF_bij_2} @{thm F.set_map(4)} @{context}\<close>)
   done
 
 lemma F'_map_cong_[fundef_cong]:
@@ -961,7 +691,7 @@ lemma F'_in_rel:
         eqTrueI[OF prems(5)]
         eqTrueI[OF supp_id_bound] eqTrueI[OF bij_id] o_apply)
     apply (subst Abs_F'_inverse[unfolded mem_Collect_eq])
-     apply (rule nonrep2_mapF_bij_2; (rule prems Rep_F'[unfolded mem_Collect_eq])?)
+     apply (rule nonrep_mapF_bij_2; (rule prems Rep_F'[unfolded mem_Collect_eq])?)
 
 (* instantiation for bounds B, frees F, lives A: [_ * nr_BFs @ id * nr_BFs @ _ * nr_As @ id * nr_As] *)
     apply (subst F.map_comp[of _ _ id id _ _ id id, unfolded o_id id_o, symmetric]; (rule prems bij_id supp_id_bound)?)
@@ -980,7 +710,7 @@ lemma F'_in_rel:
       apply ((subst Abs_F'_inverse[unfolded mem_Collect_eq]), (tactic \<open>defer_tac 1\<close>))+ 
          apply (tactic \<open>distinct_subgoals_tac\<close>)
       prefer 2
-       apply (rule nonrep2_map_F_rev; (rule bij_id supp_id_bound)?)
+       apply (rule nonrep_map_F_rev; (rule bij_id supp_id_bound)?)
        apply (subst F.map_comp; (rule bij_id supp_id_bound)?)
        apply (unfold o_id id_o)
        apply (subst subprems)
@@ -1013,13 +743,13 @@ lemma F'_in_rel:
     subgoal premises subprems for z
       apply (rule exI)
       apply (subst Abs_F'_inverse[unfolded mem_Collect_eq])
-       apply (rule nonrep2_mapF_bij_2; (rule supp_id_bound bij_id Rep_F'[unfolded mem_Collect_eq])?)
+       apply (rule nonrep_mapF_bij_2; (rule supp_id_bound bij_id Rep_F'[unfolded mem_Collect_eq])?)
       apply (rule conjI; (rule conjI)?)
 
         prefer 3(* subgoal 3 is solvable without the exI instantiation and it "instantiates" ?z 
           so that the other 2 subgoals are solvable as well*)
         apply (subst Abs_F'_inverse[unfolded mem_Collect_eq])
-         apply (rule nonrep2_mapF_bij_2; (rule prems Rep_F'[unfolded mem_Collect_eq])?)
+         apply (rule nonrep_mapF_bij_2; (rule prems Rep_F'[unfolded mem_Collect_eq])?)
         apply (subst F.map_comp; (rule bij_id supp_id_bound prems)?) (*having the id prems before the actual prems is important!*)
         apply (unfold o_id)
         apply (unfold o_def)
