operations/Linearize_orig.thy
@@ -192,9 +192,6 @@ lift_definition set2_F' :: "('a1::var,'a2::var,'a3::var,'a4) F' \<Rightarrow> 'a
 lift_definition set3_F' :: "('a1::var,'a2::var,'a3::var,'a4) F' \<Rightarrow> 'a3 set" is set3_F .
 lift_definition set4_F' :: "('a1::var,'a2::var,'a3::var,'a4) F' \<Rightarrow> 'a4 set" is set4_F .
 
-definition asSS :: "('a \<Rightarrow> 'a) \<Rightarrow> 'a \<Rightarrow> 'a" where
-  "asSS f \<equiv> if |supp f| <o |UNIV :: 'a set| then f else id"
-
 lift_definition map_F' :: "('a1::var \<Rightarrow> 'a1) \<Rightarrow> ('a2::var \<Rightarrow> 'a2) \<Rightarrow> ('a3::var \<Rightarrow> 'a3) \<Rightarrow> ('a4 \<Rightarrow> 'a4') 
   \<Rightarrow> ('a1,'a2,'a3,'a4) F' \<Rightarrow> ('a1,'a2,'a3,'a4') F'"
   is "\<lambda>v u f g. map_F (asSS v) (asSS (asBij u)) (asBij f) g" 
