operations/Linearize_rail.thy
@@ -1,0 +1,29 @@
+theory Linearize_rail
+  imports "Binders.MRBNF_Composition" "Binders.MRBNF_Recursor"
+  keywords "linearize_mrbnf" :: thy_goal
+begin
+
+ML_file "../Tools/mrbnf_linearize_tactics.ML"
+ML_file "../Tools/mrbnf_linearize.ML"
+(* this is just to build the rail diagram for linearize_mrbnf*)
+
+ML_file \<open>~~/src/Doc/antiquote_setup.ML\<close>
+text  \<open>
+\<^rail>\<open>
+  @@{command linearize_mrbnf} @{syntax spec} name '=' term @{syntax wits}? \<newline>
+    @'on' @{syntax on_vars} @{syntax bindings}? @{syntax "morphisms"}?
+  ;
+  @{syntax_def spec}: @{syntax tfree} | '(' (((name ':')? @{syntax tfree}) + ',') ')'
+  ;
+  @{syntax_def tfree}: typefree ('::' sort)
+  ;
+  @{syntax_def wits}: '[' 'wits' ':' (term + ',') ']'
+  ;
+  @{syntax_def on_vars}: (typefree + @'and')
+  ;
+  @{syntax_def bindings}: @'for' ((('map' | 'rel' | 'pred' | 'nonrep' | 'sameShape') ':' name) +)
+  ;
+  @{syntax_def "morphisms"}: @'morphisms' name name
+\<close>
+\<close>
+end
